PhysLean/QFT/PerturbationTheory/Koszul/KoszulSign.lean
@@ -4,9 +4,9 @@ Released under Apache 2.0 license as described in the file LICENSE.
 Authors: Joseph Tooby-Smith
 -/
 module
-
 public import PhysLean.QFT.PerturbationTheory.Koszul.KoszulSignInsert
 public import PhysLean.Mathematics.List.InsertionSort
+import all PhysLean.Mathematics.List
 import all Mathlib.Data.List.Sort
 /-!
 
@@ -105,18 +105,18 @@ lemma koszulSign_insertIdx [Std.Total le] [IsTrans 𝓕 le] (φ : 𝓕) :
     rw [koszulSign]
     trans koszulSign q le (φ1 :: φs) * koszulSignInsert q le φ (φ1 :: φs)
     · ring
-    simp only [instCommGroup.eq_1, List.take_zero, ofList_empty, exchangeSign_bosonic, one_mul,
-      insertionSortEquiv, List.length_cons, Nat.succ_eq_add_one, orderedInsertEquiv, eq_mpr_eq_cast,
-      cast_eq, PhysLean.Fin.equivCons_trans, mul_eq_mul_left_iff]
-    conv_lhs =>
-      enter [2, 2, 2, 2]
+    simp only [insertionSortEquiv, List.length_cons, Nat.succ_eq_add_one, orderedInsertEquiv,
+      PhysLean.Fin.equivCons_trans, Equiv.trans_apply, PhysLean.Fin.equivCons_zero]
+    conv_rhs =>
+      enter [2,2, 2, 2]
       rw [orderedInsert_eq_insertIdx_orderedInsertPos]
-    conv_lhs =>
+    conv_rhs =>
       rhs
       erw [← ofList_take_insert]
       change 𝓢(q φ, ofList q ((List.insertionSort le (φ1 :: φs)).take
         (↑(orderedInsertPos le ((List.insertionSort le (φ1 :: φs))) φ))))
       rw [← koszulSignInsert_eq_exchangeSign_take q le]
+    rw [ofList_take_zero]
     simp
   | φ1 :: φs, n + 1, h => by
     conv_lhs =>
@@ -128,6 +128,7 @@ lemma koszulSign_insertIdx [Std.Total le] [IsTrans 𝓕 le] (φ : 𝓕) :
       simp only [List.insertIdx_succ_cons]
       simp only [List.insertionSort_cons, List.length_cons, insertionSortEquiv, Nat.succ_eq_add_one,
         Equiv.trans_apply, PhysLean.Fin.equivCons_succ]
+      erw [orderedInsertEquiv_fin_succ]
       simp only [Fin.eta, Fin.val_cast]
       rhs
       simp [orderedInsert_eq_insertIdx_orderedInsertPos]
@@ -161,20 +162,7 @@ lemma koszulSign_insertIdx [Std.Total le] [IsTrans 𝓕 le] (φ : 𝓕) :
           𝓢(q φ, ofList q ((List.insertIdx rs nro φ1).take (nro.succAbove ni))))
     swap
     · simp only [rs, nro, ni]
-      conv =>
-        enter [2, 2, 2, 2, 2, 1, 1, 2, 1]
-        rw [add_comm]
-      conv =>
-        enter [2, 2, 2, 2, 2, 1, 1]
-        change (orderedInsertEquiv le (List.insertionSort le (φs.insertIdx n φ)) φ1)
-          ((PhysLean.Fin.equivCons (insertionSortEquiv le (φs.insertIdx n φ))) ⟨n.succ, _⟩)
-        simp only [Nat.succ_eq_add_one, PhysLean.Fin.equivCons, Equiv.toFun_as_coe,
-          Equiv.invFun_as_coe, Equiv.coe_fn_mk]
-        change orderedInsertEquiv le (List.insertionSort le (φs.insertIdx n φ)) φ1
-          ((Fin.succ ∘ ⇑(insertionSortEquiv le (φs.insertIdx n φ))) ⟨n, _⟩)
-        simp only [Function.comp_apply]
-        rw [orderedInsertEquiv_fin_succ]
-      grind
+      ring
     congr 1
     simp only [Fin.succAbove]
     have hns : rs.get ni = φ := by
